concurrency/Modular/templates/giveup_specs.v
@@ -3,8 +3,8 @@ Require Import VST.floyd.proofauto.
 Require Import VST.atomics.general_locks.
 Require Import bst.giveup_template. (* giveup_template.c *)
 Require Import bst.puretree.
-Require Import bst.data_struct.
-Require Import bst.giveup_lib.
+(* Require Import bst.data_struct. *)
+Require Export bst.giveup_lib.
 Require Import VST.atomics.verif_lock_atomic.
 Require Import VST.floyd.library.
 
@@ -19,7 +19,7 @@ Proof. unfold Inhabitant; apply Pos_Infinity. Defined.
 
 Section give_up_specs.
   Context {N: NodeRep}.
-  
+
 Definition nodebox_rep (g : gname) (g_root : gname) (sh : share) (lock: val) (nb : val) :=
   EX (np: val) (lsh : share),
                 data_at sh (tptr (t_struct_node)) np nb *
@@ -42,7 +42,6 @@ Definition surely_malloc_spec :=
        RETURN (p)
        SEP (mem_mgr gv; malloc_token Ews t p * data_at_ Ews t p).
 
-
 Lemma test (pt: enum * (val * (share * (gname * node_info )))) (pt1 : node_info): True.
   Proof.
     Check (((pt.2.2.2).2).1).2.
@@ -55,76 +54,7 @@ Lemma test (pt: enum * (val * (share * (gname * node_info )))) (pt1 : node_info)
     Check pt.2.2.2.2.
     Check ((pt1.1).1).1.
     Check (pt.2.2.2).2.
-    Admitted.
-
-Definition post_traverse (b: val) x (g: gname) (e: enum) (p: val) (sh: share) (g_in: gname) (n: node_info):=
-  !!( key_in_range x (n.1).2 = true ∧
-      repable_signed (number2Z (n.1).2.1) /\ repable_signed (number2Z (n.1).2.2) /\
-      is_pointer_or_null (((n.1).1).2) /\
-      (if Val.eq (enums e) (enums NN)
-       then n.2 = Some None /\ ((n.1).1).1 = nullval
-                          else ((n.1).1).1 <> nullval)
-                        (* (match (pt.1 : enum) with
-                         | NN => pt.2.2.2.2.2 = Some None /\ ((((pt.2.2.2).2).1).1).1 = nullval
-                         | NF | F =>  ((((pt.2.2.2).2).1).1).1 <> nullval
-                        (* | NF => ((((pt.2.2.2).2).1).1).1 <> nullval *)
-                          end) *)  ) && seplog.emp * 
-  data_at Ews t_struct_pn (p, p) b * in_tree g g_in p ((n.1).1).2 * node_lock_inv_pred g p g_in n.
-
-(*
-Program Definition traverse_spec :=
-  DECLARE _traverse
-          ATOMIC TYPE (rmaps.ConstType
-                       (val * val * val * Z  * val * globals * gname * gname))
-          OBJ M INVS ∅
-  WITH b, n, lock, x, v, gv, g, g_root
-  PRE [ tptr t_struct_pn, tint]
-  PROP (and (Z.le (Int.min_signed) x) (Z.le x (Int.max_signed)); is_pointer_or_null v)
-  PARAMS (b; Vint (Int.repr x)) GLOBALS (gv)
-  SEP  (mem_mgr gv; 
-        in_tree g g_root n lock;
-        !!(is_pointer_or_null lock /\ is_pointer_or_null n) && seplog.emp;
-        EX (p: val), data_at Ews (t_struct_pn) (p, n) b ) | (CSS g g_root M)
-  POST [ tint ]
-  EX  pt: enum * (val * (share * (gname * node_info ))) %type,
-  PROP ()
-  LOCAL (temp ret_temp (enums pt.1))
-  SEP (mem_mgr gv; !!( key_in_range x (((pt.2.2.2).2).1).2 = true ∧
-                         repable_signed (number2Z (((pt.2.2.2).2).1).2.1) ∧
-                         repable_signed (number2Z (((pt.2.2.2).2).1).2.2) /\
-                         is_pointer_or_null ((((pt.2.2.2).2).1).1).2
-                       /\ (if Val.eq (enums pt.1) (enums NN) then
-                            pt.2.2.2.2.2 = Some None /\ ((((pt.2.2.2).2).1).1).1 = nullval
-                          else ((((pt.2.2.2).2).1).1).1 <> nullval)
-                        (* (match (pt.1 : enum) with
-                         | NN => pt.2.2.2.2.2 = Some None /\ ((((pt.2.2.2).2).1).1).1 = nullval
-                         | NF | F =>  ((((pt.2.2.2).2).1).1).1 <> nullval
-                        (* | NF => ((((pt.2.2.2).2).1).1).1 <> nullval *)
-                          end) *)  ) && seplog.emp; 
-        data_at Ews t_struct_pn (pt.2.1, pt.2.1) b;
-        in_tree g pt.2.2.2.1 pt.2.1 ((((pt.2.2.2).2).1).1).2;
-       node_lock_inv_pred g pt.2.1 pt.2.2.2.1 (pt.2.2.2).2)| (CSS g g_root M).
-*)
-
-Program Definition traverse_spec :=
-  DECLARE _traverse
-          ATOMIC TYPE (rmaps.ConstType
-                       (val * val * val * Z  * val * globals * gname * gname))
-          OBJ M INVS ∅
-  WITH b, n, lock, x, v, gv, g, g_root
-  PRE [ tptr t_struct_pn, tint]
-  PROP (and (Z.le (Int.min_signed) x) (Z.le x (Int.max_signed)); is_pointer_or_null v)
-  PARAMS (b; Vint (Int.repr x)) GLOBALS (gv)
-  SEP  (mem_mgr gv; 
-        in_tree g g_root n lock;
-        !!(is_pointer_or_null lock /\ is_pointer_or_null n) && seplog.emp;
-        EX (p: val), data_at Ews (t_struct_pn) (p, n) b  ) | (CSS g g_root M)
-  POST [ tint ]
-  EX  pt: enum * (val * (share * (gname * node_info ))) %type,
-  PROP ()
-  LOCAL (temp ret_temp (enums pt.1))
-  SEP (mem_mgr gv; post_traverse b x g pt.1 pt.2.1 pt.2.2.1 pt.2.2.2.1 (pt.2.2.2).2)| (CSS g g_root M).
-
+Admitted.
 
 (* t_struct_node represents for the generic-struct rather specific-data-structure *)
 (* Spec of inrange function *)
@@ -157,7 +87,7 @@ Lemma node_rep_valid_pointer t g g_current p: node_rep p g g_current t |-- valid
 Proof.
   unfold node_rep.
   Intros.
-  iIntros "(((((H & ?) & ?) & ?) & ?) & ?)".
+  iIntros "((((((? & H) & ?) & ?) & ?) & ?) & ?)".
   iPoseProof (field_at_valid_ptr0 with "H") as "H"; try auto; simpl; try lia.
   iVST. entailer !.
 Qed.
@@ -232,8 +162,8 @@ Definition fst_frth_list: list (val * val * val * val) -> list (val * val) :=
   map (fun '(x, _, _, y) => (x, y)).
 
 
-Definition post_insert_giveup1 (p pnt : val) (x: Z) v
-  min max (trl : list (val * val * val * val)) g :=
+Definition post_insert_giveup1 (p pnt : val) (x: Z) v min max
+  (trl : list (val * val * val * val)) g :=
        iter_sepcon (fun pn => malloc_token Ews t_struct_node pn) (fst_list trl) * 
        iter_sepcon (fun pn => field_at Ews t_struct_node (DOT _t) (Vlong (Int64.repr 0)) pn)
          (fst_list trl) * 
@@ -249,8 +179,8 @@ Definition post_insert_giveup1 (p pnt : val) (x: Z) v
        field_at Ews t_struct_node (DOT _min) (vint min) p * 
        field_at Ews t_struct_node (DOT _max) (vint max) p.
 
-Definition post_insert_giveup2 (p pnt tp: val) (x: Z) v 
-  min max (trl : list (val * val * val * val)) (r: node_info) g :=
+Definition post_insert_giveup2 (p pnt tp: val) (x: Z) v min max
+  (trl : list (val * val * val * val)) (r: node_info) g :=
        iter_sepcon (fun pn => malloc_token Ews t_struct_node pn) (fst_list trl) * 
        iter_sepcon (fun pn => field_at Ews t_struct_node (DOT _t) tp pn)
          (fst_list trl) * 
@@ -275,10 +205,10 @@ Definition insertOp_giveup_spec :=
   PARAMS (p; Vint (Int.repr x); v; Vint (Int.repr stt))
   GLOBALS (gv)
   SEP (mem_mgr gv;
-       match (Int.eq (Int.repr stt) (Int.repr 2%Z)) with
-        | true => (!!(tp = nullval /\ (r.2 = Some None) ) && seplog.emp)
-        | false => (!!(tp <> nullval) && seplog.emp)
-       end;
+       (match (Int.eq (Int.repr stt) (Int.repr 2%Z)) with
+        | true => !!(tp = nullval /\ (r.2 = Some None)) 
+        | false => !!(tp <> nullval)
+       end) && seplog.emp *
        field_at Ews t_struct_node (DOT _t) tp p;
        field_at Ews t_struct_node (DOT _min) (vint min) p;
        field_at Ews t_struct_node (DOT _max) (vint max) p;
@@ -293,7 +223,6 @@ Definition insertOp_giveup_spec :=
         | _    => (post_insert_giveup2 p pnt tp x v min
                    max trl r g)
         end)).
-
 
 (* same as insertOp_giveup_spec, only renaming name *)
 Definition insertOp_helper_spec :=
@@ -305,10 +234,10 @@ Definition insertOp_helper_spec :=
   PARAMS (p; Vint (Int.repr x); v; Vint (Int.repr stt))
   GLOBALS (gv)
   SEP (mem_mgr gv;
-       match (Int.eq (Int.repr stt) (Int.repr 2%Z)) with
-        | true => (!!(tp = nullval /\ (r.2 = Some None) ) && seplog.emp)
-        | false => (!!(tp <> nullval) && seplog.emp)
-       end;
+       (match (Int.eq (Int.repr stt) (Int.repr 2%Z)) with
+        | true => !!(tp = nullval /\ (r.2 = Some None)) 
+        | false => !!(tp <> nullval)
+       end) && seplog.emp *
        field_at Ews t_struct_node (DOT _t) tp p;
        field_at Ews t_struct_node (DOT _min) (vint min) p;
        field_at Ews t_struct_node (DOT _max) (vint max) p;
@@ -324,11 +253,99 @@ Definition insertOp_helper_spec :=
                    max trl r g)
         end)).
 
+Definition getLock_spec :=
+  DECLARE _getLock
+    WITH p: val, lk: val, lsh : share
+  PRE [ tptr t_struct_node]
+  PROP (readable_share lsh; is_pointer_or_null lk)
+  PARAMS (p)
+  GLOBALS ()
+  SEP (field_at lsh t_struct_node (DOT _lock) lk p)
+  POST[ tptr (Tstruct _atom_int noattr) ]
+    PROP ()
+    RETURN (lk)
+    SEP (field_at lsh t_struct_node (DOT _lock) lk p ).
+
+(* FOUND = 0, NOTFOUND = 1, NULLNEXT = 2 (NULLNEXT = NULL || NEXT ) *)
+
+Definition post_traverse (b: val) x (g: gname) (e: enum) (p: val)
+  (sh: share) (g_in: gname) (r: node_info):=
+  !!( key_in_range x (r.1).2 = true ∧
+      repable_signed (number2Z (r.1).2.1) /\ repable_signed (number2Z (r.1).2.2) /\
+      is_pointer_or_null (((r.1).1).2) /\
+        (match e with
+         | NN => r.2 = Some None /\ ((r.1).1).1 = nullval
+         | NF => ((r.1).1).1 <> nullval
+         | F =>  r.2 = Some None /\ ((r.1).1).1 = nullval
+         end)) && seplog.emp *
+  data_at Ews t_struct_pn (p, p) b * in_tree g g_in p ((r.1).1).2 * node_lock_inv_pred g p g_in r.
+
+Program Definition traverse_spec :=
+  DECLARE _traverse
+          ATOMIC TYPE (rmaps.ConstType
+                       (val * val * val * Z  * val * globals * gname * gname))
+          OBJ M INVS ∅
+  WITH b, n, lock, x, v, gv, g, g_root
+  PRE [ tptr t_struct_pn, tint]
+  PROP (and (Z.le (Int.min_signed) x) (Z.le x (Int.max_signed)); is_pointer_or_null v)
+  PARAMS (b; Vint (Int.repr x)) GLOBALS (gv)
+  SEP  (mem_mgr gv; 
+        in_tree g g_root n lock;
+        !!(is_pointer_or_null lock /\ is_pointer_or_null n) && seplog.emp;
+        EX (p: val), data_at Ews (t_struct_pn) (p, n) b  ) | (CSS g g_root M)
+  POST [ tint ]
+  EX pt: enum * (val * (share * (gname * node_info ))) %type,
+  PROP ()
+  LOCAL (temp ret_temp (enums pt.1))
+  SEP (mem_mgr gv; post_traverse b x g pt.1 pt.2.1 pt.2.2.1 pt.2.2.2.1 (pt.2.2.2).2)| (CSS g g_root M).
+
+(*
+Program Definition traverse_spec :=
+  DECLARE _traverse
+          ATOMIC TYPE (rmaps.ConstType
+                       (val * val * val * Z  * val * globals * gname * gname))
+          OBJ M INVS ∅
+  WITH b, n, lock, x, v, gv, g, g_root
+  PRE [ tptr t_struct_pn, tint]
+  PROP (and (Z.le (Int.min_signed) x) (Z.le x (Int.max_signed)); is_pointer_or_null v)
+  PARAMS (b; Vint (Int.repr x)) GLOBALS (gv)
+  SEP  (mem_mgr gv; 
+        in_tree g g_root n lock;
+        !!(is_pointer_or_null lock /\ is_pointer_or_null n) && seplog.emp;
+        EX (p: val), data_at Ews (t_struct_pn) (p, n) b ) | (CSS g g_root M)
+  POST [ tint ]
+  EX  pt: enum * (val * (share * (gname * node_info ))) %type,
+  PROP ()
+  LOCAL (temp ret_temp (enums pt.1))
+  SEP (mem_mgr gv; !!( key_in_range x (((pt.2.2.2).2).1).2 = true ∧
+                         repable_signed (number2Z (((pt.2.2.2).2).1).2.1) ∧
+                         repable_signed (number2Z (((pt.2.2.2).2).1).2.2) /\
+                         is_pointer_or_null ((((pt.2.2.2).2).1).1).2
+                       /\ (if Val.eq (enums pt.1) (enums NN) then
+                            pt.2.2.2.2.2 = Some None /\ ((((pt.2.2.2).2).1).1).1 = nullval
+                          else ((((pt.2.2.2).2).1).1).1 <> nullval)
+                        (* (match (pt.1 : enum) with
+                         | NN => pt.2.2.2.2.2 = Some None /\ ((((pt.2.2.2).2).1).1).1 = nullval
+                         | NF | F =>  ((((pt.2.2.2).2).1).1).1 <> nullval
+                        (* | NF => ((((pt.2.2.2).2).1).1).1 <> nullval *)
+                          end) *)  ) && seplog.emp; 
+        data_at Ews t_struct_pn (pt.2.1, pt.2.1) b;
+        in_tree g pt.2.2.2.1 pt.2.1 ((((pt.2.2.2).2).1).1).2;
+       node_lock_inv_pred g pt.2.1 pt.2.2.2.1 (pt.2.2.2).2)| (CSS g g_root M).
+*)
 
 Definition Gprog : funspecs :=
-    ltac:(with_library prog [acquire_spec; release_spec; makelock_spec; findnext_spec; insertOp_giveup_spec; 
-                             inRange_spec; traverse_spec; 
-                             surely_malloc_spec; insertOp_helper_spec ]).
+    ltac:(with_library prog [acquire_spec; release_spec; makelock_spec; findnext_spec;
+                             insertOp_giveup_spec;
+                             inRange_spec; traverse_spec; getLock_spec;
+                             surely_malloc_spec; insertOp_helper_spec
+         ]).
+
+Lemma getLock: semax_body Vprog Gprog f_getLock getLock_spec.
+Proof.
+  start_function.
+  forward. forward.
+Qed.
 
 Lemma insertOp_helper: semax_body Vprog Gprog f_insertOp_helper insertOp_helper_spec.
 Proof.
@@ -339,5 +356,496 @@ Proof.
   Exists pnt.2.
   entailer !.
 Qed.
+
+(*
+(* traverse invariants *)
+Definition traverse_inv (b: val) (n pnN': val) (sh: share)
+                        (x : Z) (v: val) (g_root: gname) (lock: val) gv
+                        (inv_names : invariants.invG) (g : gname) AS : environ -> mpred :=
+  (EX (pnN p: val) (gN_in: gname) (lockN_in: val),
+            PROP ()
+            LOCAL (temp _p pnN'; temp _status (vint 2); temp _pn__2 b; temp _x (vint x);
+                   (* temp _value v; *) gvars gv)
+            SEP (data_at sh (t_struct_pn) (p, pnN) b;
+                 in_tree g gN_in pnN lockN_in; in_tree g g_root pnN' lock;
+                 !!(is_pointer_or_null lockN_in) && seplog.emp; AS; mem_mgr gv))%assert.
+
+Definition traverse_inv_1 (b p: val) (sh: share) (x : Z) (g_root g_in g: gname) (r: node_info) :=
+  data_at sh (t_struct_pn) (p, p) b * in_tree g g_in p r.1.1.2 *
+  node_lock_inv_pred g p g_in r *
+  (!!(key_in_range x r.1.2 = true (* /\ r.2 = Some None *) /\
+      repable_signed (number2Z r.1.2.1) ∧
+      repable_signed (number2Z r.1.2.2) /\ is_pointer_or_null r.1.1.2) && seplog.emp).
+
+Definition traverse_inv_2 (b p: val) (sh : share) (x : Z) (g_root g_in g: gname) (r: node_info) :=
+  data_at sh (t_struct_pn) (p, p) b *
+  in_tree g g_in p r.1.1.2 *
+  (* node_lock_inv_pred_1 g p g_in r x * *) (* modify it later*)
+  (!!(repable_signed (number2Z r.1.2.1) ∧
+      repable_signed (number2Z r.1.2.2) /\ is_pointer_or_null r.1.1.2) && seplog.emp).
+
+
+(* PROVING traverse spec *)
+Lemma traverse: semax_body Vprog Gprog f_traverse traverse_spec.
+Proof.
+  start_function.
+  Intros p.
+  forward.
+  forward.
+  set (AS := atomic_shift _ _ _ _ _ ).
+  (* New pt: bool * (val * (share * (gname * node_info))) *)
+  forward_loop (traverse_inv b n n Ews x v g_root lock gv inv_names g AS)
+    break: (*consider to remove gsh *)
+    (EX (flag: enum) (q : val) (gsh: share) (g_in: gname) (r: node_info),
+     PROP() LOCAL(temp _status (enums flag))
+     SEP((match flag with
+            | F => ((traverse_inv_2 b q Ews x g_root g_in g r) *
+                      (!!(r.1.1.1 <> nullval) && seplog.emp))
+            | NF => ((traverse_inv_2 b q Ews x g_root g_in g r) *
+                      (!!(r.1.1.1 <> nullval) && seplog.emp))
+            | NN => ((traverse_inv_1 b q Ews x g_root g_in g r) *
+                      (!!( r.1.1.1 = nullval) && seplog.emp)) end) *
+                       Q (flag, (q, (gsh, (g_in, r)))) * mem_mgr gv)).
+  - unfold traverse_inv.
+    Exists n p g_root lock. sep_apply in_tree_duplicate. entailer !. 
+  - (*go deeply into loop*) (*pre-condition*)
+    unfold traverse_inv.
+    Intros pn p1 g_in lock_in.
+    gather_SEP AS (in_tree g g_in pn lock_in).
+    viewshift_SEP 0 (AS * (in_tree g g_in pn lock_in) *
+                          (EX lsh, !!(readable_share lsh) &&
+                                     field_at lsh t_struct_node (DOT _lock) lock_in pn)).
+    { go_lower. apply lock_alloc. }
+    Intros lsh.
+    forward.
+    forward.
+    sep_apply in_tree_duplicate.
+    (* acquire(pn->n->lock); *)
+    forward_call acquire_inv_atomic (lock_in,
+        AS  * (EX R, node_lock_inv_pred g pn g_in R)  ).
+    {
+      iIntros "[[[[[[HITlkin HITlkin1] HAS] H4] H5] HITlkin2] H7]".
+      iCombine "HITlkin HAS" as "HITlkin".
+      iCombine "HITlkin HITlkin1 H4 H5 HITlkin2 H7" as "HITAS".
+      iVST.
+      apply sepcon_derives; [| cancel_frame].
+      unfold atomic_shift. iIntros "AU". iAuIntro; unfold atomic_acc; simpl.
+      iDestruct "AU" as "[#HITlkin AU]".
+      iMod "AU" as (m) "[Hm HClose]".
+      iModIntro.
+      iPoseProof (in_tree_inv g g_in g_root with "[$HITlkin $Hm]") as "InvLock".
+      iDestruct "InvLock" as "(InvLock & _)".
+      iDestruct "InvLock" as (r) "[H1 H2]".
+      iExists _. iFrame.
+      iSplit; iFrame.
+      iIntros "H1".
+      iSpecialize ("H2" with "H1").
+      iFrame "HITlkin".
+      iDestruct "HClose" as "[HClose _]".
+      iSpecialize ("HClose" with "H2"); auto.
+      iIntros (m') "((H1 & H1') & _)".
+      iSpecialize ("H2" with "H1").
+      iDestruct "HClose" as "[HClose _]".
+      iSpecialize ("HClose" with "H2").
+      iMod ("HClose").
+      iFrame "HClose". by iExists _.
+    }
+    Intros r.
+    forward.
+    forward.
+    unfold node_lock_inv_pred, node_rep.
+    Intros.
+    forward.
+    (* inrange function *)
+    forward_call(x, pn, (number2Z r.1.2.1), (number2Z r.1.2.2), Ews, gv).
+    Intros succ1.
+    assert_PROP(is_pointer_or_null r.1.1.1). entailer !.
+    destruct succ1.
+    + forward_if.
+      forward.
+      forward.
+      (*tp = nullval --- pn->p->t == NULL; break*)
+      forward_if.
+      (* prove r.1.1.2 = lock_in *)
+      gather_SEP (in_tree g g_in pn r.1.1.2) (in_tree g g_in pn lock_in).
+      assert_PROP (r.1.1.2 = lock_in) as Hlk.
+      { sep_apply in_tree_equiv; entailer !. }
+      Intros.
+      rewrite Hlk.
+      (* push back lock into invariant *)
+      gather_SEP AS (in_tree g g_in pn lock_in) (field_at lsh t_struct_node _ _ pn).
+      viewshift_SEP 0 (AS * (in_tree g g_in pn lock_in)).
+      {
+        go_lower.
+        iIntros "((AU & #H) & H1)".
+        iMod "AU" as (m) "[Hm HClose]".
+        iPoseProof (in_tree_inv g g_in g_root with "[$H $Hm]") as "InvLock".
+        iDestruct "InvLock" as "(_ & InvLock)".
+        iDestruct "InvLock" as (R) "[H1' H2']".
+        unfold ltree.
+        iDestruct "H1'" as (lsh1) "(%H12 & (H12 & H13))".
+        iAssert(EX lsh0 : share,
+           !! (field_compatible t_struct_node [] pn ∧ readable_share lsh0 ) &&
+           (@field_at CompSpecs lsh0 t_struct_node (DOT _lock) lock_in pn *
+               inv_for_lock lock_in R))
+               with "[H1 H12 H13]" as "H1'".
+        {
+          destruct H12 as (Hf & Hrs).
+          iPoseProof (lock_join with "[H1 H12]") as "H1".
+          { iSplitL "H1"; iFrame; iPureIntro; auto. }
+          iDestruct "H1" as (Lsh) "(% & H1)".
+          iExists _. iFrame; iPureIntro; repeat (split; auto).
+        }
+        iSpecialize ("H2'" with "H1'").
+        iDestruct "HClose" as "(HClose & _)".
+        iSpecialize ("HClose" with "H2'").
+        iMod "HClose". by iFrame.
+      }
+      viewshift_SEP 0 (EX y, Q y * (in_tree g g_in pn lock_in) *
+                               (!!(y = (NN, (pn, (Ews, (g_in, r))))) && seplog.emp)).
+      {
+        go_lower.
+        iIntros "(AU & #HITlkin)".
+        iMod "AU" as (m) "[Hm HClose]".
+        iDestruct "HClose" as "[_ HClose]".
+        iSpecialize ("HClose" $! (NN, (pn, (Ews, (g_in, r))))).
+        iFrame "HITlkin".
+        iMod ("HClose" with "[Hm]") as "Hm".
+        iFrame "Hm".
+        iModIntro. iExists _.
+        by iFrame "Hm".
+      }
+      (*proving it satisfies with the post condition of traverse *)
+      Intros y.
+      forward.
+      forward.
+      Exists NN pn Ews g_in r.
+      unfold traverse_inv_1.
+      unfold node_lock_inv_pred, node_rep.
+      entailer !.
+      destruct (r.1.2).
+      eapply key_range; auto.
+      by iIntros "(H & _)". 
+      forward.
+      assert_PROP(field_compatible t_struct_pn (DOT _n) b). entailer !.
+      forward.
+      (* findNext *)
+      forward_call(x, r.1.1.1, (field_address t_struct_pn [StructField _n] b),
+                   pn, r, g, Ews, gv).
+      { unfold_data_at (data_at Ews t_struct_pn _ b). cancel. entailer !. }
+      {
+        Intros succ.
+        (* assert_PROP(r.1.1.1 <> nullval) by entailer !. *)
+        destruct succ.1.1; last first.
+        Intros. 
+        * (* NN => succ.1.2 = succ.2  *)
+          (* not found and find the next point *)
+          forward.
+          forward_if.
+          easy. (* contradiction *)
+          forward_if.
+          easy. (* contradiction *)
+          forward.
+          gather_SEP (in_tree g g_in pn r.1.1.2) (in_tree g g_in pn lock_in).
+          assert_PROP (r.1.1.2 = lock_in) as Hlk.
+          { sep_apply in_tree_equiv; entailer !. }
+          rewrite Hlk.
+          Intros.
+          forward.
+          (* push back lock into invariant *)
+          gather_SEP AS (in_tree g g_in pn lock_in) (field_at lsh t_struct_node _ _ pn).
+          viewshift_SEP 0 (AS * (in_tree g g_in pn lock_in)).
+          { go_lower.
+            apply push_lock_back; auto.  }
+          (* make in_tree of next node : in_tree g succ.2 pnext lknext *)
+          Intros.
+          gather_SEP AS (in_tree g g_in pn lock_in) (node_rep_R r.1.1.1 r.1.2 r.2 g)
+                        (field_at _ _ _ _ pn)
+                        (field_at Ews t_struct_node _ _ pn)
+                        (field_at Ews t_struct_node _ _ pn)
+                        (malloc_token Ews t_struct_node pn) (my_half g_in Tsh r).
+          viewshift_SEP 0 (EX g_in1 lock1, AS * (node_lock_inv_pred g pn g_in r ) *
+                                           (in_tree g g_in1 succ.2 lock1)).
+          {
+            go_lower.
+            iIntros "(((((((AU & #H) & HNode) & H2) & H3) & H4) & H5) & H6)".
+            iMod "AU" as (m) "[Hm HClose]".
+            iPoseProof (ghost_update_step g g_in g_root pn succ.1.2 lock_in m r
+                         with "[$H $Hm $HNode $H2 $H3 $H4 $H5 $H6]")
+              as (g_in1 lock1) "((Inv & H1) & H2)".
+            { rewrite <- Hlk. iFrame "H". done. }
+            iExists g_in1, lock1.
+            iSpecialize ("HClose" with "H1").
+            rewrite H11.
+            by iFrame "Inv H2".
+          }
+          (*Now we have in_tree g succ.2 pnext lknext *)
+          Intros gnext lknext.
+          (* _release(_t'8);) *)
+          forward_call release_inv (lock_in, node_lock_inv_pred g pn g_in r, AS).
+          {
+            lock_props.
+            iIntros "(((((((HAS & H1) & H2) & H3) & H4) & H5) & H6) & H7)".
+            iCombine "HAS H1 H3 H2 H4 H5 H6 H7" as "Hnode_inv_pred".
+            iVST.
+            rewrite <- H11.
+            rewrite <- 2sepcon_assoc; rewrite <- 2sepcon_comm.
+            apply sepcon_derives; [| cancel_frame].
+            unfold atomic_shift;
+              iIntros "((AU & H1) & #H2)";
+
+              iAuIntro; unfold atomic_acc; simpl.
+            iMod "AU" as (m) "[Hm HClose]".
+            iModIntro.
+            iExists tt.
+            iPoseProof (in_tree_inv' g g_in g_root pn (r.1.1.2) m r
+                         with "[H2 H1 $Hm]") as "(HI1 & HI2)".
+            { rewrite Hlk. iFrame "H1 H2". }
+            iDestruct "HI1" as "(HI1' & HI1)".
+            rewrite Hlk.
+            iFrame "HI1' HI1".
+            iSplit.
+            {
+              iIntros "(Hnode_Iinv & InvLock)".
+              iSpecialize ("HI2" with "InvLock").
+              iDestruct "HClose" as "[HClose _]".
+              iFrame "Hnode_Iinv".
+              iSpecialize ("HClose" with "HI2").
+              iFrame.
+            }
+            iIntros (_) "(H & _)".
+            iSpecialize ("HI2" with "H").
+            iDestruct "HClose" as "[HClose _]". 
+            by iSpecialize ("HClose" with "HI2").
+         }
+         (* proving |--  traverse_inv *)
+         unfold traverse_inv.
+         Exists succ.1.2 pn gnext lknext.
+         entailer !. admit. (* is_pointer_or_null lknext *)
+         unfold_data_at (data_at Ews t_struct_pn _ b).
+         cancel. 
+       * (* NF case *)
+         forward.
+         forward_if.
+         forward.
+         easy.
+         forward_if.
+         gather_SEP (in_tree g g_in pn r.1.1.2) (in_tree g g_in pn lock_in).
+         assert_PROP (r.1.1.2 = lock_in) as Hlk.
+         { sep_apply in_tree_equiv; entailer !. }
+         Intros.
+         rewrite Hlk.
+         (* push back lock into invariant *)
+         gather_SEP AS (in_tree g g_in pn lock_in) (field_at lsh t_struct_node _ _ pn).
+         viewshift_SEP 0 (AS * (in_tree g g_in pn lock_in)).
+         {
+           go_lower.
+           iIntros "((AU & #H) & H1)".
+           iMod "AU" as (m) "[Hm HClose]".
+           iPoseProof (in_tree_inv g g_in g_root with "[$H $Hm]") as "InvLock".
+           iDestruct "InvLock" as "(_ & InvLock)".
+           iDestruct "InvLock" as (R) "[H1' H2']".
+           unfold ltree.
+           iDestruct "H1'" as (lsh1) "(%K12 & (H12 & H13))".
+           iAssert(EX lsh0 : share,
+                      !! (field_compatible t_struct_node [] pn ∧ readable_share lsh0 ) &&
+                        (@field_at CompSpecs lsh0 t_struct_node (DOT _lock) lock_in pn *
+               inv_for_lock lock_in R))
+               with "[H1 H12 H13]" as "H1'".
+        {
+          destruct K12 as (Hf & Hrs).
+          iPoseProof (lock_join with "[H1 H12]") as "H1".
+          { iSplitL "H1"; iFrame; iPureIntro; auto. }
+          iDestruct "H1" as (Lsh) "(% & H1)".
+          iExists _. iFrame; iPureIntro; repeat (split; auto).
+        }
+        iSpecialize ("H2'" with "H1'").
+        iDestruct "HClose" as "(HClose & _)".
+        iSpecialize ("HClose" with "H2'").
+        iMod "HClose". by iFrame.
+      }
+      viewshift_SEP 0 (EX y, Q y * (in_tree g g_in pn lock_in) *
+                               (!!(y = (NF, (succ.1.2, (Ews, (g_in, r))))) && seplog.emp)).
+      {
+        go_lower.
+        iIntros "(AU & #HITlkin)".
+        iMod "AU" as (m) "[Hm HClose]".
+        iDestruct "HClose" as "[_ HClose]".
+        iSpecialize ("HClose" $! (NF, (succ.1.2, (Ews, (g_in, r))))).
+        iFrame "HITlkin".
+        iMod ("HClose" with "[Hm]") as "Hm".
+        iFrame "Hm".
+        iModIntro. iExists _.
+        by iFrame "Hm".
+      }
+      Intros y.
+      rewrite <- H11.
+      forward.
+      forward.
+      Exists NF succ.1.2 Ews g_in r.
+      unfold traverse_inv_2.
+      entailer !.
+      unfold_data_at (data_at Ews t_struct_pn _ b).
+      cancel.
+      admit.
+      (* re-modify traverse_inv_2 *)
+      (* contradiction *)
+      easy.
+    * forward.
+      forward_if.
+      gather_SEP (in_tree g g_in pn r.1.1.2) (in_tree g g_in pn lock_in).
+      assert_PROP (r.1.1.2 = lock_in) as Hlk.
+      { sep_apply in_tree_equiv; entailer !. }
+      Intros.
+      rewrite Hlk.
+      (* push back lock into invariant *)
+      gather_SEP AS (in_tree g g_in pn lock_in) (field_at lsh t_struct_node _ _ pn).
+      viewshift_SEP 0 (AS * (in_tree g g_in pn lock_in)).
+      {
+        go_lower.
+        iIntros "((AU & #H) & H1)".
+        iMod "AU" as (m) "[Hm HClose]".
+        iPoseProof (in_tree_inv g g_in g_root with "[$H $Hm]") as "InvLock".
+        iDestruct "InvLock" as "(_ & InvLock)".
+        iDestruct "InvLock" as (R) "[H1' H2']".
+        unfold ltree.
+        iDestruct "H1'" as (lsh1) "(%K12 & (H12 & H13))".
+        iAssert(EX lsh0 : share,
+                      !! (field_compatible t_struct_node [] pn ∧ readable_share lsh0 ) &&
+                        (@field_at CompSpecs lsh0 t_struct_node (DOT _lock) lock_in pn *
+               inv_for_lock lock_in R))
+               with "[H1 H12 H13]" as "H1'".
+        {
+          destruct K12 as (Hf & Hrs).
+          iPoseProof (lock_join with "[H1 H12]") as "H1".
+          { iSplitL "H1"; iFrame; iPureIntro; auto. }
+          iDestruct "H1" as (Lsh) "(% & H1)".
+          iExists _. iFrame; iPureIntro; repeat (split; auto).
+        }
+        iSpecialize ("H2'" with "H1'").
+        iDestruct "HClose" as "(HClose & _)".
+        iSpecialize ("HClose" with "H2'").
+        iMod "HClose". by iFrame.
+      }
+      viewshift_SEP 0 (EX y, Q y * (in_tree g g_in pn lock_in) *
+                               (!!(y = (F, (succ.1.2, (Ews, (g_in, r))))) && seplog.emp)).
+      {
+        go_lower.
+        iIntros "(AU & #HITlkin)".
+        iMod "AU" as (m) "[Hm HClose]".
+        iDestruct "HClose" as "[_ HClose]".
+        iSpecialize ("HClose" $! (F, (succ.1.2, (Ews, (g_in, r))))).
+        iFrame "HITlkin".
+        iMod ("HClose" with "[Hm]") as "Hm".
+        iFrame "Hm".
+        iModIntro. iExists _.
+        by iFrame "Hm".
+      }
+      Intros y.
+      rewrite <- H11.
+      forward.
+      forward.
+      Exists F succ.1.2 Ews g_in r.
+      unfold traverse_inv_2.
+      (* re-modify traverse_inv_2 *)
+      admit.
+      (* contradiction *)
+      easy.
+    }
+    easy.
+  + forward_if.
+    easy.
+    forward.
+    forward.
+    gather_SEP (in_tree g g_in pn r.1.1.2) (in_tree g g_in pn lock_in).
+    assert_PROP (r.1.1.2 = lock_in) as Hlk.
+    { sep_apply in_tree_equiv; entailer !. }
+    rewrite Hlk.
+    Intros.
+      (* push back lock into invariant *)
+    gather_SEP AS (in_tree g g_in pn lock_in) (field_at lsh t_struct_node _ _ pn).
+    viewshift_SEP 0 (AS * (in_tree g g_in pn lock_in)).
+    { go_lower; apply push_lock_back; auto. }
+    Intros.
+    gather_SEP AS (in_tree g g_in pn lock_in) (node_rep_R r.1.1.1 r.1.2 r.2 g)
+                        (field_at _ _ _ _ pn)
+                        (field_at Ews t_struct_node _ _ pn)
+                        (field_at Ews t_struct_node _ _ pn)
+                        (malloc_token Ews t_struct_node pn) (my_half g_in Tsh r).
+    viewshift_SEP 0 (AS * (node_lock_inv_pred g pn g_in r )).
+    {
+            go_lower.
+            iIntros "(((((((AU & #H) & HNode) & H2) & H3) & H4) & H5) & H6)".
+            iFrame.
+            rewrite <- Hlk. iFrame "H". done.
+    }
+    forward_call release_inv (lock_in, node_lock_inv_pred g pn g_in r, AS).
+    {
+        lock_props.
+        iIntros "(((((HAS & H1) & H2) & H3) & H4) & H5)".
+        iCombine "HAS H1 H2 H3 H4 H5" as "Hnode_inv_pred".
+        iVST.
+        rewrite <- 2sepcon_assoc; rewrite <- 2sepcon_comm.
+        apply sepcon_derives; [| cancel_frame].
+        unfold atomic_shift; iIntros "((AU & H1) & #H2)";
+
+              iAuIntro; unfold atomic_acc; simpl.
+        iMod "AU" as (m) "[Hm HClose]".
+        iModIntro.
+        iExists tt.
+        iPoseProof (in_tree_inv' g g_in g_root pn (r.1.1.2) m r
+                         with "[H2 H1 $Hm]") as "(HI1 & HI2)".
+        { rewrite Hlk. iFrame "H1 H2". }
+          iDestruct "HI1" as "(HI1' & HI1)".
+          rewrite Hlk.
+          iFrame "HI1' HI1".
+          iSplit.
+          {
+            iIntros "(Hnode_Iinv & InvLock)".
+            iSpecialize ("HI2" with "InvLock").
+            iDestruct "HClose" as "[HClose _]".
+            iFrame "Hnode_Iinv".
+            iSpecialize ("HClose" with "HI2").
+              iFrame.
+          }
+          iIntros (_) "(H & _)".
+          iSpecialize ("HI2" with "H").
+          iDestruct "HClose" as "[HClose _]". 
+          by iSpecialize ("HClose" with "HI2").
+     }
+     (* proving |--  traverse_inv *)
+       forward.
+       unfold traverse_inv.
+       Exists n pn g_root lock.
+       sep_apply (in_tree_duplicate g g_root n).
+       entailer !. 
+    - (* semax Delta (PROP ( )  RETURN ( ) SEP ()) (return _flag;) POSTCONDITION *)
+       Intros flag.
+       Intros pn gsh g_in r.
+       unfold traverse_inv_1, traverse_inv_2.
+       destruct flag.
+       (*
+       + simpl.
+         autorewrite with norm.
+         forward.
+         unfold post_traverse.
+         Exists (true, (pn, (gsh, (g_in, r)))).
+         simpl. entailer !. 
+       + forward.
+         Exists (false, (pn, (gsh, (g_in, r)))).
+         simpl.
+         unfold node_lock_inv_pred_1, node_rep_1 at 1, tree_rep_R_1 at 1.
+         Intros g1 g2 v1 p1 p2 l1 l2.
+         rewrite H7.
+         entailer !.
+         exists v1, g1, g2; auto.
+         unfold node_lock_inv_pred, node_rep, tree_rep_R.
+         rewrite -> if_false; auto.
+         simpl.
+         Exists g1 g2 x v1 p1 p2 l1 l2.
+         entailer !. apply derives_refl.
+Qed.
+*)
+*)
 
 End give_up_specs.
